update the example & delete unused code

compcertox/ClightPLink.v
@@ -9,18 +9,7 @@ Import ClightP.
 
 Set Asymmetric Patterns.
 
-Definition link_privvar (v1 v2: list (ident * privvar))
-  (vs: list (ident * globdef fundef type))
-  : True + { v | v = v1 ++ v2
-              /\ list_disjoint (map fst v1) (map fst v2)
-              /\ list_disjoint (map fst v) (map fst vs) }.
-Proof.
-  destruct (list_disjoint_dec ident_eq (map fst v1) (map fst v2)).
-  destruct (list_disjoint_dec ident_eq (map fst (v1 ++ v2)) (map fst vs)).
-  - right. eexists (v1 ++ v2). split; eauto.
-  - left. easy.
-  - left. easy.
-Defined.
+Opaque PTree_Properties.of_list.
 
 Definition link_program (p1 p2: program): option program :=
   match link (program_of_program p1) (program_of_program p2) with
@@ -34,9 +23,11 @@ Definition link_program (p1 p2: program): option program :=
                   p1.(prog_comp_env) p2.(prog_comp_env)
                   p1.(prog_comp_env_eq) p2.(prog_comp_env_eq) EQ with
           | exist env (conj P Q) =>
-              match link_privvar p1.(prog_private) p2.(prog_private) p.(AST.prog_defs) with
-              | inl _ => None
-              | inr (exist privs (conj _ (conj p1 p2))) =>
+              let privs := p1.(prog_private) ++ p2.(prog_private) in
+              match list_norepet_dec peq
+                      ((map fst privs ++ map fst p.(AST.prog_defs))) with
+              | right _ => None
+              | left H =>
                   Some {| prog_private := privs;
                          prog_defs := p.(AST.prog_defs);
                          prog_public := p.(AST.prog_public);
@@ -44,8 +35,8 @@ Definition link_program (p1 p2: program): option program :=
                          prog_types := typs;
                          prog_comp_env := env;
                          prog_comp_env_eq := P;
-                         prog_disjoint := p2;
-                         |}
+                         prog_norepet := H;
+                       |}
               end
           end
       end
@@ -79,25 +70,23 @@ Next Obligation.
   destruct (link_build_composite_env (prog_types x) (prog_types y) typs
               (prog_comp_env x) (prog_comp_env y) (prog_comp_env_eq x)
               (prog_comp_env_eq y) EQ) as (env & P & Q & R).
-  destruct (link_privvar (prog_private x) (prog_private y)) as [l|] eqn:LV; try discriminate.
+  destruct list_norepet_dec; try discriminate.
   destruct (link_linkorder _ _ _ LP).
   intros X; inv X.
-  unfold link_privvar in LV.
-  destruct (list_disjoint_dec ident_eq (map fst (prog_private x)) (map fst (prog_private y))); try discriminate.
-  destruct (list_disjoint_dec ident_eq (map fst (prog_private x ++ prog_private y)) (map fst (AST.prog_defs p))); try discriminate.
-  inv LV. inv H2.
-  split; split; auto. 1-2: split; auto.
-  - cbn -[PTree_Properties.of_list].
-    intros * Hx. rewrite ptree_of_list_app_none; eauto.
-    destruct (lift_option ((PTree_Properties.of_list (prog_private y)) ! id)) as [[w Hw]|]; eauto.
+  split; split; auto. 1-2: split; auto; cbn.
+  - intros * Hx. rewrite ptree_of_list_app_none; eauto.
+    destruct ((PTree_Properties.of_list (prog_private y)) ! id)
+      eqn: Hw; eauto.
     exfalso.
     apply PTree_Properties.in_of_list in Hx.
     apply PTree_Properties.in_of_list in Hw.
-    eapply list_disjoint_notin. apply l. instantiate (1 := id).
+    apply list_norepet_append_left in l.
+    rewrite map_app in l.
+    apply list_norepet_app in l as (A1 & A2 & A3).
+    eapply list_disjoint_notin. apply A3. instantiate (1 := id).
     apply in_map_iff. eexists (_, _). split; eauto. easy.
     apply in_map_iff. eexists (_, _). split; eauto. easy.
-  - cbn -[PTree_Properties.of_list].
-    intros * Hx. erewrite ptree_of_list_app; eauto.
+  - intros * Hx. erewrite ptree_of_list_app; eauto.
 Qed.
 
 Transparent Linker_prog.
@@ -114,32 +103,34 @@ Proof.
     cbn. eauto.
 Qed.
 
-Lemma ptree_of_list_map {A B} (f: A -> B) xs id b:
-  (PTree_Properties.of_list
-     (map (fun '(id, x) => (id, f x)) xs)) ! id = Some b <->
-    (exists a, (PTree_Properties.of_list xs) ! id = Some a /\ f a = b).
-Proof.
-  induction xs as [| [id' a]].
-  - cbn. split. intros. inv H. intros (a & Ha & ?). inv Ha.
-  - cbn. destruct (ListDec.In_dec PTree.elt_eq id (map fst xs)).
-    + setoid_rewrite ptree_of_list1; eauto.
-      apply in_map_iff in i as ((x & y) & Hx & Hy). cbn in *. subst.
-      apply in_map_iff. eexists (_, _); split; eauto. reflexivity.
-      apply in_map_iff. eexists (_, _); split; eauto.
-    + setoid_rewrite ptree_of_list2; eauto.
-      * destruct (peq id id').
-        -- subst. setoid_rewrite PTree.gss. split.
-           ++ intros. inv H. eexists; split; eauto.
-           ++ intros (a' & Ha & Hb). subst. congruence.
-        -- setoid_rewrite PTree.gso; eauto.
-           setoid_rewrite PTree.gempty.
-           split; intros; try congruence.
-           destruct H; easy.
-      * intros c. apply n.
-        apply in_map_iff in c as ((x & y) & Hx & Hy). cbn in *. subst.
-        apply in_map_iff in Hy as ((x & z) & Hx & Hz). inv Hx.
-        apply in_map_iff. eexists (_, _); split; eauto. reflexivity.
-Qed.
+(* Lemma ptree_of_list_map {A B} (f: A -> B) xs id b: *)
+(*   (PTree_Properties.of_list *)
+(*      (map (fun '(id, x) => (id, f x)) xs)) ! id = Some b <-> *)
+(*     (exists a, (PTree_Properties.of_list xs) ! id = Some a /\ f a = b). *)
+(* Proof. *)
+(*   induction xs as [| [id' a]]. *)
+(*   - cbn. split. intros. inv H. intros (a & Ha & ?). inv Ha. *)
+(*   - cbn. destruct (ListDec.In_dec PTree.elt_eq id (map fst xs)). *)
+(*     + setoid_rewrite ptree_of_list1; eauto. *)
+(*       apply in_map_iff in i as ((x & y) & Hx & Hy). cbn in *. subst. *)
+(*       apply in_map_iff. eexists (_, _); split; eauto. reflexivity. *)
+(*       apply in_map_iff. eexists (_, _); split; eauto. *)
+(*     + setoid_rewrite ptree_of_list2; eauto. *)
+(*       * destruct (peq id id'). *)
+(*         -- subst. setoid_rewrite PTree.gss. split. *)
+(*            ++ intros. inv H. eexists; split; eauto. *)
+(*            ++ intros (a' & Ha & Hb). subst. congruence. *)
+(*         -- setoid_rewrite PTree.gso; eauto. *)
+(*            setoid_rewrite PTree.gempty. *)
+(*            split; intros; try congruence. *)
+(*            destruct H; easy. *)
+(*       * intros c. apply n. *)
+(*         apply in_map_iff in c as ((x & y) & Hx & Hy). cbn in *. subst. *)
+(*         apply in_map_iff in Hy as ((x & z) & Hx & Hz). inv Hx. *)
+(*         apply in_map_iff. eexists (_, _); split; eauto. reflexivity. *)
+(* Qed. *)
+
+Import PTree_Properties.
 
 Lemma linkorder_erase:
   forall (p q: program), linkorder p q ->
@@ -147,38 +138,184 @@ Lemma linkorder_erase:
 Proof.
   intros * ((A1 & A2 & A3) & B & C).
   split. apply A1. split. apply A2.
-  intros *  H1. destruct p, q.
-  unfold prog_defmap in *.
-  cbn -[PTree_Properties.of_list] in *.
-  destruct (lift_option ((PTree_Properties.of_list (map (fun '(id, g) => (id, erase_globdef g)) prog_defs0)) ! id)) as [[w Hw]|].
+  intros * H1. destruct p, q.
+  unfold prog_defmap in *. cbn in *.
+  unfold prog_defmap in *. cbn in *.
+  rewrite of_list_elements in *.
+  destruct ((of_list prog_defs0) ! id) eqn: Hw;
+    destruct ((of_list prog_private0) ! id) eqn: Hu;
+    rewrite PTree.gcombine in H1 by reflexivity;
+    rewrite Hw in H1; rewrite Hu in H1; cbn in H1; inv H1.
   (* normal variables *)
-  - erewrite ptree_of_list_app in H1; eauto. inv H1.
-    apply ptree_of_list_map in Hw as (v & Hv1 & Hv2). subst.
-    specialize (A3 _ _ Hv1).
-    destruct A3 as (u & Hu1 & Hu2 & Hu3).
-    exists (erase_globdef u). split. 2: split.
-    + erewrite ptree_of_list_app; eauto.
-      eapply ptree_of_list_map. eexists; split; eauto.
+  - specialize (A3 _ _ Hw) as (x & Hx1 & Hx2 & Hx3).
+    exists (erase_globdef x). split. 2: split.
+    + rewrite PTree.gcombine. 2: reflexivity.
+      rewrite Hx1.
+      destruct ((of_list prog_private1) ! id) eqn: Hy.
+      * exfalso.
+        apply list_norepet_app in prog_norepet1 as (?&?&Ha).
+        eapply Ha; eauto. instantiate (1 := id).
+        apply in_of_list in Hy. apply in_map_iff.
+        eexists (_, _). split; eauto. reflexivity.
+        apply in_of_list in Hx1. apply in_map_iff.
+        eexists (_, _). split; eauto. reflexivity.
+      * reflexivity.
     + apply globdef_linkorder_erase; eauto.
-    + intros Hp. rewrite Hu3; eauto.
+    + intros Hp. rewrite Hx3; eauto.
   (* private variable *)
-  - erewrite ptree_of_list_app_none in H1; eauto.
-    apply ptree_of_list_map in H1 as (v & Hv1 & Hv2). subst.
-    specialize (C _ _ Hv1).
-    eexists (clightp_erase_privvar v). split. 2: split.
-    + erewrite ptree_of_list_app_none.
-      * apply ptree_of_list_map. eexists; split; eauto.
-      * apply PTree_Properties.in_of_list in C.
-        assert (D: In id (map fst prog_private1)).
-        apply in_map_iff. eexists (_, _); split; eauto. reflexivity.
-        destruct (lift_option (PTree_Properties.of_list (map (fun '(id0, g) => (id0, erase_globdef g)) prog_defs1)) ! id) as [[q Hq]|]; eauto.
-        exfalso.
-        apply PTree_Properties.in_of_list in Hq.
-        apply in_map_iff in Hq as ((id' & x) & Hr1 & Hr2). inv Hr1.
-        eapply prog_disjoint1.
-        apply in_map_iff. eexists (_, _); split; eauto.
-        apply in_map_iff. eexists (_, _); split; eauto.
-        reflexivity.
-    + apply linkorder_refl.
-    + intros. reflexivity.
+  - specialize (C _ _ Hu).
+    eexists (clightp_erase_privvar p). split. 2: split.
+    + rewrite PTree.gcombine. 2: reflexivity.
+      rewrite C.
+      destruct ((of_list prog_defs1) ! id) eqn: Hy.
+      * exfalso.
+        apply list_norepet_app in prog_norepet1 as (?&?&Ha).
+        eapply Ha; eauto. instantiate (1 := id).
+        apply in_of_list in C. apply in_map_iff.
+        eexists (_, _). split; eauto. reflexivity.
+        apply in_of_list in Hy. apply in_map_iff.
+        eexists (_, _). split; eauto. reflexivity.
+      * reflexivity.
+    + reflexivity.
+    + easy.
+Qed.
+
+Inductive clightp_link_rel:
+  option privvar -> option privvar ->
+  option (globdef fundef type) -> option (globdef fundef type) -> Prop :=
+| clightp_link_rel0: clightp_link_rel None None None None
+| clightp_link_rel1 p: clightp_link_rel (Some p) None None None
+| clightp_link_rel2 p: clightp_link_rel None (Some p) None None
+| clightp_link_rel3 p: clightp_link_rel None None (Some p) None
+| clightp_link_rel4 p: clightp_link_rel None None None (Some p)
+| clightp_link_rel5 p1 p2: clightp_link_rel None None (Some p1) (Some p2).
+
+Hint Resolve in_of_list.
+
+Lemma clightp_link_rel_intro (p1 p2: program):
+  (forall id g1 g2,
+      (of_list (prog_defs p1)) ! id = Some g1 ->
+      (of_list (prog_defs p2)) ! id = Some g2 ->
+      (exists g, link g1 g2 = Some g)) ->
+  list_norepet
+    (map fst (prog_private p1 ++ prog_private p2) ++
+       map fst
+       (PTree.elements
+          (PTree.combine link_prog_merge (prog_defmap p1) (prog_defmap p2)))) ->
+  forall id : positive,
+    clightp_link_rel (of_list (prog_private p1)) ! id
+      (of_list (prog_private p2)) ! id
+      (of_list (prog_defs p1)) ! id
+      (of_list (prog_defs p2)) ! id.
+Proof.
+  intros Hg H id.
+  assert
+    (HX: forall a b c d,
+      (of_list (prog_private p1)) ! id = Some a \/
+      (of_list (prog_private p2)) ! id = Some b ->
+      (of_list (prog_defs p1)) ! id = Some c \/
+      (of_list (prog_defs p2)) ! id = Some d -> False).
+  {
+    intros * Hp Hd.
+    assert (In id (map fst (PTree.elements (PTree.combine link_prog_merge (prog_defmap p1) (prog_defmap p2))))).
+    {
+      Ltac link_rel_solve1 H1 H2 :=
+        split; eauto;
+        apply PTree.elements_correct;
+        rewrite PTree.gcombine by reflexivity;
+        setoid_rewrite H1;
+        setoid_rewrite H2; eauto.
+      destruct ((of_list (prog_defs p1)) ! id) eqn: Hd1;
+        destruct ((of_list (prog_defs p2)) ! id) eqn: Hd2.
+      - specialize (Hg _ _ _ Hd1 Hd2) as (gx & Hg).
+        apply in_map_iff. eexists (id, gx).
+        link_rel_solve1 Hd1 Hd2.
+      - destruct Hd; try congruence. inv H0.
+        apply in_map_iff. eexists (id, c).
+        link_rel_solve1 Hd1 Hd2.
+      - destruct Hd; try congruence. inv H0.
+        apply in_map_iff. eexists (id, d).
+        link_rel_solve1 Hd1 Hd2.
+      - destruct Hd; congruence.
+    }
+    assert (In id (map fst (prog_private p1 ++ prog_private p2))).
+    {
+      rewrite map_app. apply in_or_app.
+      destruct Hp; [ left | right ]; apply in_map_iff.
+      - eexists (id, a). split; eauto.
+      - eexists (id, b). split; eauto.
+    }
+    apply list_norepet_app in H as (A & B & C).
+    eapply C; eauto.
+  }
+  Ltac lr_solve H :=
+    exfalso; eapply H; solve [ left; eauto | right; eauto ].
+  destruct ((of_list (prog_private p1)) ! id) eqn: Hp1;
+    destruct ((of_list (prog_private p2)) ! id) eqn: Hp2.
+  - exfalso. apply list_norepet_app in H as (A & B & C).
+    rewrite map_app in A.
+    apply list_norepet_app in A as (A1 & A2 & A3).
+    eapply A3; eauto; apply in_map_iff.
+    + eexists (id, p). split; eauto.
+    + eexists (id, p0). split; eauto.
+  - destruct ((of_list (prog_defs p1)) ! id) eqn: Hd1;
+      destruct ((of_list (prog_defs p2)) ! id) eqn: Hd2;
+      try lr_solve HX.
+    constructor.
+  - destruct ((of_list (prog_defs p1)) ! id) eqn: Hd1;
+      destruct ((of_list (prog_defs p2)) ! id) eqn: Hd2;
+      try lr_solve HX.
+    constructor.
+  - destruct ((of_list (prog_defs p1)) ! id) eqn: Hd1;
+      destruct ((of_list (prog_defs p2)) ! id) eqn: Hd2;
+      constructor.
+Unshelve. all: eauto.
+Qed.
+
+Lemma link_clightp_erase (p1 p2 p: program):
+  link p1 p2 = Some p ->
+  link (clightp_erase_program p1) (clightp_erase_program p2) =
+    Some (clightp_erase_program p).
+Proof.
+  intros Hp. unfold link in *. cbn in *.
+  unfold link_program in Hp.
+  destruct link eqn: H1; try congruence.
+  destruct lift_option as [[x H2]|]; try congruence.
+  destruct link_build_composite_env as (env & H3 & H4 & H5).
+  destruct list_norepet_dec; try congruence.
+  apply link_prog_inv in H1 as (Hmain & Hdef & Hp0).
+  rewrite link_prog_succeeds.
+  - inv Hp. f_equal.
+    unfold clightp_erase_program. cbn in *. f_equal.
+    unfold prog_defmap. cbn.
+    apply PTree.elements_extensional. intros id.
+    rewrite !PTree.gcombine by reflexivity.
+    rewrite !of_list_elements.
+    rewrite !PTree.gcombine by reflexivity.
+    apply clightp_link_rel_intro with (id:=id) in l.
+    2: { intros * Hx Hy. eapply Hdef; eauto. }
+    Ltac rewrite_none H :=
+      rewrite ptree_of_list_app_none; eauto; rewrite <- H.
+    inv l; cbn; try (rewrite_none H0; reflexivity).
+    + erewrite ptree_of_list_app; eauto. reflexivity.
+    + rewrite_none H0. cbn.
+      exploit Hdef. 1-2: symmetry; eauto.
+      intros (?&?&(gd & Hgd)). rewrite Hgd.
+      apply link_erase_globdef; eauto.
+  - apply Hmain.
+  - unfold clightp_erase_program, prog_defmap. cbn.
+    setoid_rewrite of_list_elements.
+    intros * HA HB.
+    subst p0. cbn in l. clear Hp.
+    apply clightp_link_rel_intro with (id:=id) in l.
+    2: { intros * Hx Hy. eapply Hdef; eauto. }
+    rewrite PTree.gcombine in HA, HB by reflexivity.
+    inv l; cbn; rewrite <- H0 in HA; rewrite <- H in HB;
+      rewrite <- H6 in HA; rewrite <- H7 in HB;
+      cbn in *; try congruence.
+    exploit Hdef. 1-2: symmetry; eauto.
+    intros (A & B & (gd & Hgd)). repeat split; eauto.
+    inv HA; inv HB.
+    apply link_erase_globdef in Hgd; eauto.
+    rewrite Hgd. discriminate.
 Qed.
